\documentclass[11pt, a4paper]{article}
\usepackage{amsmath, fullpage}

\begin{document}

\begin{align*}
    y & = mx + b           \\
    m & = \text{slope}     \\
    b & = \text{intercept}
\end{align*}

\begin{align*}
    \text{Given matrices:}                                                \\
    x                               & =
    \begin{bmatrix}
        x_1 \\
        x_2 \\
        x_3 \\
    \end{bmatrix}
    \text{and y = }
    \begin{bmatrix}
        y_1 \\
        y_2 \\
        y_3 \\
    \end{bmatrix}                                                        \\
    \text{The equation in matrix form: }                                  \\
    y                               & = mx + b                            \\
    y =
    \begin{bmatrix}
        y_1 \\
        y_2 \\
        y_3 \\
    \end{bmatrix}
    =
    \begin{bmatrix}
        1 & x_1 \\
        1 & x_2 \\
        1 & x_3 \\
    \end{bmatrix}
                                    & \cdot
    \begin{bmatrix}
        b \\ m
    \end{bmatrix}
    =
    \begin{bmatrix}
        b + mx_1 \\
        b + mx_2 \\
        b + mx_3 \\
    \end{bmatrix}                                                        \\ \\
    X B                             & = Y                                 \\
    \left(X^T X\right)^{-1} X^T X B & = \left(X^T X\right)^{-1} X^T Y     \\
    B                               & = \left(X^T X\right)^{-1} X^T Y     \\
    \text{Where:}                                                         \\
    X^T    \text{ represents }      & \text{the transpose of matrix } X.  \\
    X^{-1} \text{ represents }      & \text{the inverse of matrix }    X. \\
\end{align*}


\begin{align*}
    BIC_k & = n \,\, ln(SSE) + k \,\, ln(x) \\ \\
    \text{Where,}                           \\
    k     & = degree                        \\
    SSE   & = \text{sum of squared errors}  \\
    n     & = \text{number of data points}
\end{align*}

\begin{align*}
    MSE       & = \frac{1}{n} \sum_{i = 1}^{n} (Y_i - \hat{Y}_i)^2 \\ \\
    \text{Where,}                                                  \\
    n         & = \text{number of data points}                     \\
    Y_i       & = \text{real values}                               \\
    \hat{Y}_i & = \text{predicted values}
\end{align*}


\begin{align*}
    \text{You can rewrite MSE as}                                                                               \\
    MSE                                        & = \frac{1}{n} \sum_{i = 1}^{n} (y_i - (m \, x_i + b))^2        \\
    \text{let, } f(m, b)                       & = (y_i - (m \, x_i + b))^2                                     \\
    \text{let, }  g(m, b)                      & = y_i - (m x_i + b)                                            \\
    \text{so, } f(m, b)                        & = g(m, b)^2                                                    \\
    \text{Partial derivative w.r.t m,}                                                                          \\
    \frac{\partial f}{\partial m}              & = 2 \, g(m, b) \cdot  \frac{\partial g}{\partial m}            \\
    \text{now, } \frac{\partial g}{\partial m} & = 0 - (1\, x_i + 0)                                            \\
                                               & = -\, x_i                                                      \\
    \text{expanding, }                                                                                          \\
    \frac{\partial f}{\partial m}              & = 2 \, (y_i - (m\, x_i + b)) \, \cdot (-x_i)                   \\
                                               & = -2\, x_i \cdot (y_i - (m\, x_i + b))                         \\
    \text{Partial derivative w.r.t b,}                                                                          \\
    \frac{\partial f}{\partial b}              & = 2 \, g(m, b) \cdot \frac{\partial g}{\partial b}                 \\
    \text{now, } \frac{\partial g}{\partial b} & = 0 - (0\cdot 0 + 1)                                           \\
                                               & = -1                                                           \\
    \text{expanding, }                                                                                          \\
    \frac{\partial f}{\partial b}              & = 2 \cdot (y_i - (m\,x_i + b))^2 \cdot -1                      \\
                                               & = -2\, (y_i - (m\,x_i + b))                                    \\ \\
    \text{Final answer, }                                                                                       \\
    \frac{\partial}{\partial m}                & = \frac{2}{n} \, \sum_{i = 1}^{n} \, -x_i (y_i - (m\,x_i + b)) \\
    \frac{\partial}{\partial b}                & = \frac{2}{n} \, \sum_{i = 1}^{n} \, -(y_i - (m\,x_i + b))
\end{align*}

\end{document}
